

## An Operator Method.

Let  $x$  be an  $n$ -times differentiable function of the independent variable  $t$ . We denote the operation of differentiation with respect to  $t$  by the symbol  $D$  and call  $D$  a differential operator. So

$$Dx \equiv \frac{dx}{dt}, \quad D^2x \equiv \frac{d^2x}{dt^2}, \quad \dots \quad D^n x \equiv \frac{d^n x}{dt^n}$$

Further extending this operator notation,

$$(D+c)x \equiv \frac{dx}{dt} + cx \quad \text{and} \quad (aD^n + bD^m)x = a \frac{d^n x}{dt^n} + b \frac{d^m x}{dt^m}.$$

In this notation

$$a_0 \frac{d^n x}{dt^n} + a_1 \frac{d^{n-1} x}{dt^{n-1}} + \dots + a_{n-1} \frac{dx}{dt} + a_n x$$

can be written

$$(a_0 D^n + a_1 D^{n-1} + \dots + a_{n-1} D + a_n)x.$$

Example Consider the linear differential operator

$$3D^2 + 5D - 2$$

and  $x = t^3$ . We have, since  $\frac{dx}{dt} = 3t^2$   $\frac{d^2x}{dt^2} = 6t$

$$(3D^2 + 5D - 2)x = 18t + 15t^2 - t^3$$

We denote the operator  $a_0 D^n + a_1 D^{n-1} + \dots + a_{n-1} D + a_n$  by  $L$ , that is  $L \equiv a_0 D^n + \dots + a_n$ .

Now suppose that  $f_1$  and  $f_2$  are both  $n$ -times differentiable functions of  $t$  and  $c_1, c_2$  are constants. It is easy to show that

$$L(c_1 f_1 + c_2 f_2) = c_1 Lf_1 + c_2 Lf_2.$$

Now let  $L_1 \equiv \sum_{i=0}^n a_i D^{n-i}$  and  $L_2 \equiv \sum_{j=0}^n b_j D^{n-j}$

be two linear differential operators. Let  $L_1(r) = \sum_{i=0}^n a_i r^{n-i}$

and  $L_2(r) = \sum_{j=0}^n b_j r^{n-j}$  be the two polynomials in  $r$ . Let us denote

the product of the polynomial  $L_1(r)$  and  $L_2(r)$  by  $L(r)$ ; that is

$$L(r) = L_1(r) \cdot L_2(r).$$

Then, if  $f$  is a function possessing  $n$ th derivatives, it can be shown that

$$L_1 L_2 f = L_2 L_1 f = L f.$$

We now consider a linear system of the form.

$$L_1 x + L_2 y = f_1(t) \quad (I).$$

$$L_3 x + L_4 y = f_2(t)$$

where  $L_1 \equiv \sum_{i=0}^m a_i D^{m-i}$ ,  $L_2 \equiv \sum_{j=0}^n b_j D^{n-j}$ ,  $L_3 \equiv \sum_{k=0}^p \alpha_k D^{p-k}$

and  $L_4 \equiv \sum_{l=0}^q \beta_l D^{q-l}$

A simple example of a system which may be expressed in the form (I).

For example

$$2 \frac{dx}{dt} - 2 \frac{dy}{dt} - 3x = t \Rightarrow 2 \frac{dx}{dt} - 3x - 2 \frac{dy}{dt} = t$$

$$2 \frac{dx}{dt} + 2 \frac{dy}{dt} + 3x + 8y = 2 \Rightarrow 2 \frac{dx}{dt} + 3x + 2 \frac{dy}{dt} + 8y = 2.$$

$$\Rightarrow (2D-3)x - 2Dy = t$$

$$(2D+3)x + (2D+8)y = 2.$$

Returning the system (1), we apply the operator  $L_4$  to the first equation of (1) and the operator  $L_2$  to the second equation of (1),

obtaining

$$L_4 L_1 x + L_4 L_2 y = L_4 f_1$$

$$L_2 L_3 x + L_2 L_4 y = L_2 f_2$$

$$=$$

$$L_4 L_1 x - L_2 L_3 x = L_4 f_1 - L_2 f_2$$

Since  $L_4 L_2 = L_2 L_4$

$$(L_4 L_1 - L_2 L_3) x = L_4 f_1 - L_2 f_2.$$

or

Let  $L_5 = L_4 L_1 - L_2 L_3$  and  $g(t) = L_4 f_1 - L_2 f_2$ . Then we have

$$L_5 x = g_1$$

(2)

which is a linear differential equation with constant coefficients.

We can solve the equation  $L_S X = g_1$ .

Similarly we first obtain the equation  $L_S Y = g_2$  and then solve this equation.

Example: Solve the system  $\begin{cases} 2\frac{dx}{dt} - 2\frac{dy}{dt} - 3x = t \\ 2\frac{dx}{dt} + 2\frac{dy}{dt} + 3x + 8y = 2 \end{cases}$

Solution:  $(2D-3)X - 2DY = t \quad \backslash (2D+8)$   
 $(2D+3)X + (2D+8)Y = 2 \quad \backslash 2D$

$$\Rightarrow \begin{array}{r} (2D+8)(2D-3)X - 2D(2D+8)Y = (2D+8)t \\ + \quad 2D(2D+3)X + 2D(2D+8)Y = 2D \cdot 2 \end{array}$$

$$(4D^2 - 6D + 16D - 24 + 4D^2 + 16D)X = 2 + 8t$$

$$(8D^2 + 16D - 24)X = 8t + 2$$

$$(D^2 + 2D - 3)X = t + \frac{1}{4}$$

$$m^2 + 2m - 3 = (m+3)(m-1) = 0 \Rightarrow m = -3 \quad m = 1$$

$$y_c = C_1 e^{-3t} + C_2 e^t$$

$$y_p = At + B \Rightarrow y_p' = A \quad y_p'' = 0$$

$$\begin{array}{l} 2A - 3(At + B) = t + \frac{1}{4} \Rightarrow -3A = 1 \quad 2A - 3B = \frac{1}{4} \\ A = -\frac{1}{3} \quad B = -\frac{11}{36} \end{array}$$

$$X = C_1 e^t + C_2 e^{-3t} - \frac{1}{3}t - \frac{11}{36}$$

$$\begin{array}{r} - (2D+3)(2D-3)X + 2D(2D+3)Y = -(2D+3)t \\ + \quad (2D+3)(2D-3)X + (2D+8)(2D+3)Y = (2D+3)2 \end{array}$$

$$(4D^2 + 6D + 4D^2 - 6D + 16D - 24)Y = -2 + 3t - 6$$

$$(8D^2 + 16D - 24)Y = -3t - 8$$

$$y_p = At + B \Rightarrow 16A - 24At - 24B = -3t - 8$$

$$-24B = -10 \Rightarrow B = \frac{5}{12}$$

$$A = \frac{-3}{-24} = \frac{1}{8}$$

(3)

$$y = k_1 e^t + k_2 e^{-3t} + \frac{1}{8}t + \frac{5}{12}.$$

$\begin{vmatrix} 2D-3 & -2D \\ 2D+3 & 2D+8 \end{vmatrix} = 8D^2 + 16D - 24.$  Since this is of order two, the number of independent constant in the general solution of the system must also be two.

By substituting in the first equation.

$$\left( \frac{2k_1 e^t + 2k_2 e^{-3t} - \frac{2}{3}}{8} \right) + \left( \frac{-2k_1 e^t - 2k_2 e^{-3t} - \frac{1}{4}}{4} \right) = -3k_1 e^t - 3k_2 e^{-3t} + t + \frac{11}{12}t$$

$$(-k_1 - 2k_2)e^t + (-k_2 - 2k_1)e^{-3t} + t - \frac{2}{3} - \frac{1}{4} + \frac{11}{12} = t$$

$$(-k_1 - 2k_2)(e^t + e^{-3t}) + t = t$$

$$-k_1 - 2k_2 = 0 \quad C_1 = -2k_2 \quad \text{or} \quad k_1 = -\frac{1}{2}C_2.$$

$$(-k_2 - 2k_1) = 0 \quad C_2 = -2k_1 \quad \text{or} \quad k_2 = -\frac{1}{2}C_1.$$

The general solution

$$x = C_1 e^t + C_2 e^{-3t} - \frac{1}{3}t - \frac{11}{36}$$

$$y = -\frac{1}{2}C_1 e^t - \frac{1}{2}C_2 e^{-3t} + \frac{1}{8}t + \frac{5}{12}.$$

**B**

## Exercices

$$1) \frac{dx}{dt} + \frac{dy}{dt} - 2x - 4y = e^t$$

$$\frac{dx}{dt} + \frac{dy}{dt} - y = e^{4t}$$

$$\begin{cases} (0-2)x + (0-4)y = e^t \\ 0x + (0-1)y = e^{4t} \end{cases} \Rightarrow$$

$$\begin{aligned} (0^2 - 3 \cdot 0 + 2)x &= (0-1)e^t \\ (-0^2 + 4 \cdot 0)x &= (-0+4)e^{4t} \\ \hline (0+2)x &= 0 \end{aligned}$$

$$m+2=0 \Rightarrow m=-2 \quad \underline{\underline{x = ce^{-2t}}}$$

$$-0(0-2) + (-0^2 + 4 \cdot 0)y = -0 \cdot e^t = -e^t$$

$$(0-2)0x + (0^2 - 3 \cdot 0 + 2)y = (0-2)e^{4t} = 4e^{4t} - 2e^{4t} = 2e^{4t}$$

$$(0+2)y = 2e^{4t} - e^t \Rightarrow \frac{dy}{dt} + 2y = 2e^{4t} - e^t$$

$$0+2 \neq 0 \Rightarrow m=-2 \quad y_c = e^{-2t}$$

$$y_p = Ae^{4t} + Be^t \Rightarrow \frac{dy_p}{dt} = 4Ae^{4t} + Be^t$$

$$4Ae^{4t} + Be^t + 2Ae^{4t} + 2Be^t = 6Ae^{4t} + 3Be^t = 2e^{4t} - e^t$$

$$A = \frac{1}{3} \quad B = -\frac{1}{3}$$

$$\underline{\underline{y = ke^{-2t} + \frac{1}{3}e^{4t} - \frac{1}{3}e^t}}$$

$$\frac{dx}{dt} + \frac{dy}{dt} - 2x - 4y = e^t \Rightarrow -2ce^{-2t} + \frac{2k}{3}e^{-2t} + \frac{4}{3}e^{4t} - \frac{1}{3}e^t - 2ce^{-2t}$$

$$-4ke^{-2t} - \frac{4}{3}e^{4t} + \frac{4}{3}e^t = (-4c - 6k)e^{-2t} + e^t = e^t$$

$$(-4c - 6k) = 0 \Rightarrow k = -\frac{2}{3}c$$

$$(ce^{-2t}, -\frac{2}{3}ce^{-2t} + \frac{1}{3}e^{4t} - \frac{1}{3}e^t)$$

$$2) \frac{dx}{dt} + \frac{dy}{dt} - x = -2t$$

$$\frac{dx}{dt} + \frac{dy}{dt} - 3x - y = t^2$$

$$3) \frac{dx}{dt} + \frac{dy}{dt} + x = e^{3t}$$

$$\frac{dx}{dt} + \frac{dy}{dt} - x - 3y = e^t$$

$$(0+1)x + 0y = e^{3t}$$

$$(0-1)x + (0-3)y = e^t$$

$$\begin{matrix} 0-3 \\ -0 \end{matrix}$$

$$(0+1)(0-3)x = (0-3)e^{3t}$$

$$-0(0-1)x = (-0)e^t$$

$$(D^2 - 2D - 3)X = 0 \Rightarrow (-D - 3)X = -e^t$$

$$(-D^2 + D)X = -e^t \Rightarrow (-D - 3)X = -e^t$$

$$X_2 = ce^{-3t}$$

$$X_p = Ae^t \Rightarrow -Ae^t - 3Ae^t = -4Ae^t = -e^t \Rightarrow A = \frac{1}{4}$$

$$X = ce^{-3t} + \frac{1}{4}e^t$$

$$-(D-1)(D+1)X - D(D-1)Y = -(D-1)e^{3t} = -3e^{3t} + e^{3t} = -2e^{3t}$$

$$(D-1)(D+1)X + (D+1)(D-3)Y = (D+1)e^t = 2e^t$$

$$(-D-3)Y = -2e^{3t} + 2e^t \Rightarrow \frac{dy}{dt} + 3Y = 2e^{3t} - 2e^t$$

$$Y_p = Ae^{3t} + Be^t \Rightarrow Y_p' = 3Ae^{3t} + Be^t \Rightarrow 3Ae^{3t} + Be^t + 3Ae^{3t} + 3Be^t$$

$$= 6Ae^{3t} + 4Be^t = 2e^{3t} - 2e^t \Rightarrow A = \frac{1}{3} \quad B = -\frac{1}{2}$$

$$Y = ke^{-3t} + \frac{1}{3}e^{3t} - \frac{1}{2}e^t$$

$$-3ce^{3t} + \frac{1}{4}e^t - 3ke^{-3t} + e^{3t} - \frac{1}{2}e^t + ce^{-3t} + \frac{1}{4}e^t = e^{3t}$$

$$(-2c - 3k)e^{-3t} = 0 \Rightarrow k = -\frac{2}{3}$$

$$(-2D+1)(D+1) = -2D^2 - 2D + D + 1 = -2D^2 - D + 1$$

$$(ce^{-3t} + \frac{1}{4}e^t, -\frac{2}{3}e^{-3t} + \frac{1}{3}e^{3t} - \frac{1}{2}e^t)$$

$$4) \frac{dx}{dt} + \frac{dy}{dt} - x - 2y = 2e^t \quad \frac{dx}{dt} + \frac{dy}{dt} - 3x - 4y = e^{2t}$$

$$5) 2 \frac{dx}{dt} + \frac{dy}{dt} - x - y = e^{-t} \quad \frac{dx}{dt} + \frac{dz}{dt} + 2x + y = e^t$$

$$(2D-1)X + (D-1)Y = e^{-t} \quad | +$$

$$(D+2)X + (D+1)Y = e^t \quad | - D \times$$

$$(2D^2 + D - 1)X = -e^{-t} + e^t = 0$$

$$(-D^2 - D + 2)X = -e^t + e^t = 0$$

$$(D^2 + 1)X = 0$$

$$m^2 + 1 = 0 \quad m = \pm i$$

$$X = c_1 \sin t + c_2 \cos t$$

$$(D^2 + D - 2)Y = (D+2)e^{-t} = -e^{-t} + 2e^{-t} = e^{-t}$$

$$(-2D^2 - D + 1)Y = (-2D+1)e^t = 2e^t + e^t = 3e^t$$

(b)

16

$$(-D^2-1)y = -e^t + e^{-t} \Rightarrow (D^2+1)y = e^t - e^{-t}$$

$$y_c = k_1 \sin t + k_2 \cos t$$

$$y_p = A e^t + B e^{-t} \Rightarrow y_p'' = A e^t + B e^{-t} \Rightarrow 2A e^t + 2B e^{-t} = e^t - e^{-t}$$

$$A = \frac{1}{2} \quad B = -\frac{1}{2} \quad y = k_1 \sin t + k_2 \cos t + \frac{1}{2} e^t - \frac{1}{2} e^{-t}$$

$$(2) \Rightarrow \underline{c_1 \cos t - c_2 \sin t + k_1 \cos t - k_2 \sin t} + \frac{1}{2} e^t + \frac{1}{2} e^{-t} + \underline{2c_1 \sin t + 2c_2 \cos t}$$

$$k_1 \sin t + k_2 \cos t + \frac{1}{2} e^t - \frac{1}{2} e^{-t} = e^t$$

$$(c_1 + k_1 + 2c_2 + k_2) \cos t + (-c_2 - k_2 + 2c_1 + k_1) \sin t = 0$$

$$k_1 + k_2 = -c_1 - 2c_2$$

$$k_1 - k_2 = -2c_1 + c_2$$

$$k_1 = \frac{-3c_1 - c_2}{2}$$

$$k_2 = \frac{c_1 - 3c_2}{2}$$

$$6) \quad 2 \frac{dx}{dt} + \frac{dy}{dt} - 3x - y = t \quad 1) \quad \frac{dx}{dt} + \frac{dy}{dt} - 4x - y = e^t$$

$$(-D+1)(D-2)$$

$$-D^2 + 2D + 1D - 12$$

$$7) \quad \frac{dx}{dt} + \frac{dy}{dt} - x - 6y = e^{3t} \quad \frac{dx}{dt} + 2 \frac{dy}{dt} - 2x - 6y = t$$

$$(D-1)x + (D-6)y = e^{3t}$$

$$(2D^2 - 8D + 6)x = (2D-6)e^{3t}$$

$$(D-2)x + (2D-6)y = t$$

$$(-D^2 + 8D - 12)x = (-D+6)t$$

$$(D^2 - 6)x = 6e^{3t} - 6e^{3t} - 1 + 6t = 6t - 1$$

$$m^2 - 6 = 0 \Rightarrow m = \pm \sqrt{6} \Rightarrow x_c = c_1 e^{\sqrt{6}t} + c_2 e^{-\sqrt{6}t}$$

$$x_p = At + B \Rightarrow x_p'' = 0 \Rightarrow \frac{d^2x}{dt^2} - 6x = -6At - 6B = 6t - 1 \Rightarrow A = \frac{1}{2} \quad B = -\frac{1}{6}$$

$$x = c_1 e^{\sqrt{6}t} + c_2 e^{-\sqrt{6}t} + t + \frac{-1}{6}$$

$$(D^2 - 8D + 12)y = (D-2)e^{3t} = 3e^{3t} - 2e^{3t} = e^{3t}$$

$$(-2D^2 + 8D - 6)y = (-D+1)t = -1+t$$

$$\Rightarrow (-D^2 + 6)y = e^{3t} + t - 1$$

$$y_p = A e^{3t} + Bt + C \Rightarrow y_p'' = 9A e^{3t}$$

$$-9A e^{3t} + 6A e^{3t} + 6Bt + 6C = e^{3t} + t - 1$$

$$A = -\frac{1}{3} \quad B = \frac{1}{6} \quad C = -\frac{1}{6}$$

$$y = k_1 e^{\sqrt{6}t} + k_2 e^{-\sqrt{6}t} - \frac{e^{3t}}{3} + \frac{t}{6} - \frac{1}{6}$$

7

$$8) \frac{dx}{dt} + \frac{dy}{dt} - x - y = 1$$

$$\frac{dx}{dt} + 2 \frac{dy}{dt} - 2x - 3y = 1$$

$$9) \frac{dx}{dt} + \frac{dy}{dt} + 2y = \sin t$$

$$\frac{dx}{dt} + \frac{dy}{dt} - x - y = 0$$

$$10) \frac{dx}{dt} - \frac{dy}{dt} - 2x + 4y = t$$

$$\frac{dx}{dt} + \frac{dy}{dt} - x - y = 1$$

$$18) \frac{d^2x}{dt^2} + \frac{dy}{dt} = e^{2t}$$

$$\frac{dx}{dt} + \frac{dy}{dt} - x - y = 0$$

$$19) \frac{d^2x}{dt^2} + \frac{dy}{dt} - x + y = 1$$

$$\frac{d^2y}{dt^2} + \frac{dx}{dt} - x + y = 0$$

$$21) \frac{d^2x}{dt^2} + \frac{dy}{dt} = t + 1$$

$$\frac{dx}{dt} + \frac{dy}{dt} - 3x + y = 2t - 1$$

Solution of 19

$$(D^2 - 1)x + (D + 1)y = 1$$

$$(D^4 - 1)x = (D^2 + 1)1 = 1$$

$$(D - 1)x + (D^2 + 1)y = 0$$

$$-(D^2 - 1)x = -(D + 1)0 = 0$$

$$((D^4 - 1) - (D^2 - 1))x = (D^2 - 1)(D^2 + 1 - 1)x = D^2(D^2 - 1)x = 1$$

$$m^2(m^2 - 1) = 0 \Rightarrow m = 0, 0, -1, 1 \quad X_c = C_1 + C_2 t + C_3 e^t + C_4 e^{-t}$$

$$\frac{d^4x}{dt^4} - \frac{d^2x}{dt^2} = 1 \quad (X_p = At^2) \quad 0 - 2A = 1 \Rightarrow A = -\frac{1}{2}$$

$$X_p = \sum_{n=0}^{\infty} A_n t^n \quad X_p'' = \sum_{n=2}^{\infty} n(n-1) A_n t^{n-2} \quad X_p^{(IV)} = \sum_{n=4}^{\infty} n(n-1)(n-2)(n-3) A_n t^{n-4}$$

$$(X_p^{(IV)} - X_p'') = 1 \Leftrightarrow$$

$$X = C_1 + C_2 t + C_3 e^t + C_4 e^{-t} - \frac{t^2}{2}$$

$$(D^2 - 1)x + (D + 1)y = 1$$

$$-(D^2 - 1)x - (D + 1)(D^2 + 1)y = (D + 1)0 = 0$$

$$(D + 1)(1 - D^2 - 1)y = -D^2(D + 1)y = 1 \Rightarrow y_c = k_1 + k_2 t + k_3 e^{-t}$$

$$y_p = At^2 \Rightarrow y_p'' = 2A \quad y_p''' = 0 \Rightarrow -2A = 1 \Rightarrow A = -\frac{1}{2}$$

$$y = k_1 + k_2 t + k_3 e^{-t} - \frac{t^2}{2}$$

$$k_1 = 1 + C_1 - C_2 \quad k_2 = (1 + C_2) \quad k_3 = C_4$$

Using these values for  $k_1$  and  $k_2$  in (7.56), the resulting pair (7.54) and (7.56) constitute the general solution of the system (7.51). That is, the general solution of (7.51) is given by

$$x = c_1 e^t + c_2 e^{-3t} - \frac{1}{3}t - \frac{11}{36}$$

$$y = -\frac{1}{2}c_1 e^t + \frac{3}{2}c_2 e^{-3t} + \frac{1}{3}t + \frac{5}{12}$$

where  $c_1$  and  $c_2$  are arbitrary constants. If we had chosen  $k_1$  and  $k_2$  as the independent constants in (7.57), then the general solution of the system (7.51) would have been written

$$x = -2k_1 e^t + \frac{2}{3}k_2 e^{-3t} - \frac{1}{3}t - \frac{11}{36}$$

$$y = k_1 e^t + k_2 e^{-3t} + \frac{1}{3}t + \frac{5}{12}$$

### Exercises

Use the operator method described in this section to find the general solution of each of the following linear systems.

1.  $\frac{dx}{dt} + \frac{dy}{dt} - 2x - 4y = e^t$

2.  $\frac{dx}{dt} + \frac{dy}{dt} - x = -2t$

$\frac{dx}{dt} + \frac{dy}{dt} - y = e^{4t}$

$\frac{dx}{dt} + \frac{dy}{dt} - 3x - y = t^2$

3.  $\frac{dx}{dt} + \frac{dy}{dt} - x - 3y = e^t$

4.  $\frac{dx}{dt} + \frac{dy}{dt} - x - 2y = 2e^t$

$\frac{dx}{dt} + \frac{dy}{dt} + x = e^{3t}$

$\frac{dx}{dt} + \frac{dy}{dt} - 3x - 4y = e^{2t}$

5.  $2\frac{dx}{dt} + \frac{dy}{dt} - x - y = e^{-t}$

6.  $2\frac{dx}{dt} + \frac{dy}{dt} - 3x - y = t$

$\frac{dx}{dt} + \frac{dy}{dt} + 2x + y = e^t$

$\frac{dx}{dt} + \frac{dy}{dt} - 4x - y = e^t$

7.  $\frac{dx}{dt} + \frac{dy}{dt} - x - 6y = e^{3t}$

8.  $\frac{dx}{dt} + \frac{dy}{dt} - x - 3y = 3t$

$\frac{dx}{dt} + 2\frac{dy}{dt} - 2x - 6y = t$

$\frac{dx}{dt} + 2\frac{dy}{dt} - 2x - 3y = 1$

9.  $\frac{dx}{dt} + \frac{dy}{dt} + 2y = \sin t$

10.  $\frac{dx}{dt} - \frac{dy}{dt} - 2x + 4y = t$

$\frac{dx}{dt} + \frac{dy}{dt} - x - y = 0$

$\frac{dx}{dt} + \frac{dy}{dt} - x - y = 1$

$$\checkmark 11. 2\frac{dx}{dt} + \frac{dy}{dt} + x + 5y = 4t$$

$$\frac{dx}{dt} + \frac{dy}{dt} + 2x + 2y = 2$$

$$\checkmark 13. 2\frac{dx}{dt} + \frac{dy}{dt} + x + y = t^2 + 4t$$

$$\frac{dx}{dt} + \frac{dy}{dt} + 2x + 2y = 2t^2 - 2t$$

$$15. 2\frac{dx}{dt} + 4\frac{dy}{dt} + x - y = 3e^t$$

$$\frac{dx}{dt} + \frac{dy}{dt} + 2x + 2y = e^t$$

$$17. 2\frac{dx}{dt} + \frac{dy}{dt} - x - y = 1$$

$$\frac{dx}{dt} + \frac{dy}{dt} + 2x - y = t$$

$$\checkmark 19. \frac{d^2x}{dt^2} + \frac{dy}{dt} - x + y = 1$$

$$\frac{d^2y}{dt^2} + \frac{dx}{dt} - x + y = 0$$

$$21. \frac{d^2x}{dt^2} - \frac{dy}{dt} = t + 1$$

$$\frac{dx}{dt} + \frac{dy}{dt} - 3x + y = 2t - 1$$

$$12. \frac{dx}{dt} + \frac{dy}{dt} - x + 5y = t^2$$

$$\frac{dx}{dt} + 2\frac{dy}{dt} - 2x + 4y = 2t + 1$$

$$14. 3\frac{dx}{dt} + 2\frac{dy}{dt} - x + y = t - 1$$

$$\frac{dx}{dt} + \frac{dy}{dt} - x = t + 2$$

$$16. 2\frac{dx}{dt} + \frac{dy}{dt} - x - y = -2t$$

$$\frac{dx}{dt} + \frac{dy}{dt} + x - y = t^2$$

$$18. \frac{d^2x}{dt^2} + \frac{dy}{dt} = e^{2t}$$

$$\frac{dx}{dt} + \frac{dy}{dt} - x - y = 0$$

$$20. \frac{d^2x}{dt^2} - \frac{dy}{dt} = e^t$$

$$\frac{dx}{dt} + \frac{dy}{dt} - 4x - y = 2e^t$$

## 7.4 Applications

### A. Applications to Mechanics

Systems of linear differential equations originate in the mathematical formulation of numerous problems in mechanics. We consider one such problem in the following example. Another mechanics problem leading to a linear system is given in the exercises at the end of this section.

**Example 7.16.** On a smooth horizontal plane  $BC$  (for example, a smooth table top) an object  $A_1$  is connected to a fixed point  $P$  by a massless spring  $S_1$  of natural length  $L_1$ . An object  $A_2$  is then connected to  $A_1$  by a massless spring  $S_2$  of natural length  $L_2$  in such a way that the fixed point  $P$  and the centers of gravity  $A_1$  and  $A_2$  all lie in a straight line (see Figure 7.1).

The object  $A_1$  is then displaced a distance  $a_1$  to the right or left of its equilibrium position  $O_1$ , the object  $A_2$  is displaced a distance  $a_2$  to the right or left of its equilibrium position  $O_2$ , and at time  $t = 0$  the two objects are released (see Figure 7.2). What are the positions of the two objects at any time  $t > 0$ ?

# THE LAPLACE TRANSFORM.

Definition: let  $F$  be a real-valued function of the real variable  $t$ , defined for  $t > 0$ . let  $s$  be a variable which we shall assume to be real, and consider the function  $f$  defined by

$$f(s) = \int_0^{\infty} e^{-st} F(t) dt \quad (I)$$

for all values of  $s$  for which this integral exists. The function  $f$  defined by the integral (I) is called the Laplace Transform of the function  $F$ . We shall denote the Laplace Transform of  $F$  by  $\mathcal{L}(F)$  and shall denote  $f(s)$  by  $\mathcal{L}\{F(t)\}$ .

Examples 1) Consider the function  $F$  defined by  $F(t) = 1$ , for  $t > 0$ .

$$\begin{aligned} \mathcal{L}(1) &= \int_0^{\infty} e^{-st} \cdot 1 dt = \lim_{R \rightarrow \infty} \int_0^R e^{-st} dt = \lim_{R \rightarrow \infty} \left. -\frac{e^{-st}}{s} \right|_0^R \\ &= \left( \lim_{R \rightarrow \infty} -\frac{e^{-sR}}{s} \right) - \frac{-e^0}{s} = \frac{1}{s} \quad \text{for all } s > 0. \quad \text{Thus we have} \end{aligned}$$

$$\mathcal{L}(1) = \frac{1}{s} \quad (s > 0).$$

2)  $F(t) = t$ , for  $t > 0$ .

$$\begin{aligned} \mathcal{L}(t) &= \int_0^{\infty} e^{-st} \cdot t dt = \lim_{R \rightarrow \infty} \int_0^R e^{-st} \cdot t dt = \lim_{R \rightarrow \infty} \left. \left( -\frac{(st+1)}{s^2} \cdot e^{-st} \right) \right|_0^R \\ &= \frac{1}{s^2} - \lim_{R \rightarrow \infty} \left( \frac{(sR+1) \cdot e^{-sR}}{s^2} \right) = \frac{1}{s^2}. \quad \text{Thus we have} \end{aligned}$$

$$\mathcal{L}(t) = \frac{1}{s^2} \quad (s > 0).$$